src/tls/test/TestClient13.fst
@@ -138,486 +138,7 @@ let ffiConfig tlsversion hostname =
   } in
   state
 
-(*****************************************************************************************)
-type ffiStateServerHello = {
-    cssh_guard: string;
-    cssh_config: config;
-    cssh_ks: ks;
-    cssh_log: bytes;
-    cssh_lg: HandshakeLog.log;
-    cssh_ch: HandshakeMessages.ch;
-    }
-        
-val ffiPrepareClientHello: ffiState:ffiStateClientHello -> (cbytes * ffiStateServerHello)
-let ffiPrepareClientHello ffiState =
-  let _ = (if not (ffiState.csch_guard = "CSCH") then IO.print_string ("Incorrect csch_guard "^ffiState.csch_guard^"\n")) in
-  let config = ffiState.csch_config in
-  let ks = ffiState.csch_ks in
-  let lg = ffiState.csch_lg in
-  let log = ffiState.csch_log in
-  let (ClientHello ch,chb) = Handshake.prepareClientHello config ks lg None None in
-  let pv = ch.ch_protocol_version in
-  let kex = TLSConstants.Kex_ECDHE in
-  let (str,hs,log) = makeHSRecord pv (ClientHello ch) log in
-  let r = Record.makePacket Content.Handshake pv hs in 
-  let newstate:ffiStateServerHello = {
-        cssh_guard = "CSSH";
-        cssh_config = config;
-        cssh_ks = ks;
-        cssh_log = log;
-        cssh_lg = lg;
-        cssh_ch = ch;
-    } in
-  (get_cbytes r, newstate)
-  
-(*****************************************************************************************)
-let rec really_check buf len = 
-    let lb = length buf in
-    if len = 0 then Correct buf
-    else if len = lb then Correct buf
-    else Error(AD_illegal_parameter,  "Unexpected buffer length")
-  
-let check_read header record pv =
-  match really_check header 5 with 
-  | Correct header -> (
-      match Record.parseHeader header with  (* contenType protocolVersion length *)
-      | Correct (ct,pv,len) -> (
-         match really_check record len with
-         | Correct payload  -> Correct (ct,pv,payload)
-         | Error e          -> Error e )
-      | Error e             -> Error e )
-  | Error e                 -> Error e
-  
-let handleHSRecord header record pv kex log = 
-match check_read header record pv with
-  | Error z -> Error z
-  | Correct(Content.Handshake,rpv,pl) -> Handshake.parseHandshakeMessages (Some pv) (Some kex) pl
     
-type ffiStateCertificateVerify = {
-    cscv_guard: string;
-    cscv_config: config;
-    cscv_ks: ks;
-    cscv_log: bytes;
-    cscv_lg: HandshakeLog.log;
-    cscv_ch: HandshakeMessages.ch;
-    cscv_n:nego;
-    cscv_sh:HandshakeMessages.sh;
-    }
-
- let recvHSRecord2 header record pv kex log = 
-  let c = check_read header record pv in
-  match c with
-  | Error (x,z) -> IO.print_string (z^"\n"); failwith "error"
-  | Correct(Content.Handshake,rpv,pl) -> (
-    match Handshake.parseHandshakeMessages (Some pv) (Some kex) pl with
-    | Correct (rem,[(hs_msg,to_log)]) -> 
-     	      (IO.print_string ("Received HS("^(string_of_handshakeMessage hs_msg)^")\n");
-	       (hs_msg,log @| to_log))
-    | Error (x,z) -> IO.print_string (z^"\n"); failwith "error"
-    )
-  
- let recvCCRecord2 header record pv kex log = 
-  let c = check_read header record pv in
-  match c with
-  | Error (x,z) -> IO.print_string (z^"\n"); failwith "error"
-  | Correct(Content.Change_cipher_spec,rpv,pl) -> (
-    match Handshake.parseHandshakeMessages (Some pv) (Some kex) pl with
-    | Correct (rem,[(hs_msg,to_log)]) -> 
-     	      (IO.print_string ("Received HS("^(string_of_handshakeMessage hs_msg)^")\n");
-	       (hs_msg,log @| to_log))
-    | Error (x,z) -> IO.print_string (z^"\n"); failwith "error"
-    )
-  
-val ffiHandleServerHelloWorker: ffiState:ffiStateServerHello -> header:cbytes -> record:cbytes -> (result (ffiStateCertificateVerify))
-let ffiHandleServerHelloWorker ffiState cheader crecord =
-  let _ = (if not (ffiState.cssh_guard = "CSSH") then IO.print_string ("Incorrect cssh_guard "^ffiState.cssh_guard^"\n")) in
-  let header = abytes cheader in
-  let record = abytes crecord in
-  let config = ffiState.cssh_config in
-  let log = ffiState.cssh_log in
-  let ch = ffiState.cssh_ch in
-  let lg = ffiState.cssh_lg in
-  let ks = ffiState.cssh_ks in
-  let kex = TLSConstants.Kex_ECDHE in
-  let pv = config.maxVer in
-  let ServerHello(sh),log = recvHSRecord2 header record pv kex log in
-  let Correct (n,k) = Handshake.processServerHello config ks lg None ch (ServerHello sh,log) in
-  let newstate:ffiStateCertificateVerify = {
-        cscv_guard = "CSCV";
-        cscv_config=config;
-        cscv_ch=ch;
-        cscv_ks=ks;
-        cscv_log=log;
-        cscv_lg=lg;
-        cscv_n=n;
-        cscv_sh=sh;
-    } in Correct(newstate)
-  
-  val ffiHandleServerHello: ffiState:ffiStateServerHello -> header:cbytes -> record:cbytes -> ffiStateCertificateVerify
-  let ffiHandleServerHello ffiState cheader crecord =
-    match ffiHandleServerHelloWorker ffiState cheader crecord with
-    | Error (x,z) -> IO.print_string (z^"\n"); failwith "error"
-    | Correct (x) -> x
-     
-(*****************************************************************************************)
-type ffiStateKeyExchange = {
-    cske_guard: string;
-    cske_config: config;
-    cske_ks: ks;
-    cske_log: bytes;
-    cske_lg: HandshakeLog.log;
-    cske_ch: HandshakeMessages.ch;
-    cske_n:nego;
-    cske_sc:HandshakeMessages.crt;
-    cske_sh:HandshakeMessages.sh;
-    cske_scb:bytes;
-    }
-
-val ffiHandleCertificateVerifyWorker12: ffiState:ffiStateCertificateVerify -> header:bytes -> record:bytes -> (result (ffiStateKeyExchange))
-let ffiHandleCertificateVerifyWorker12 ffiState header record =
-  let _ = (if not (ffiState.cscv_guard = "CSCV") then IO.print_string ("Incorrect cssh_guard "^ffiState.cscv_guard^"\n")) in
-  let config = ffiState.cscv_config in
-  let log = ffiState.cscv_log in
-  let sh = ffiState.cscv_sh in
-  let n = ffiState.cscv_n in
-  let pv = n.n_protocol_version in
-  let cs = n.n_cipher_suite in
-  let CipherSuite kex sa ae = cs in
-  match pv with
-    | TLS_1p2 -> (let (Certificate(sc),scb) = recvHSRecord2 header record pv kex log in
-                     IO.print_string ("Certificate validation status = " ^
-                       (if Cert.validate_chain sc.crt_chain true config.peer_name config.ca_file then
-                       "OK" else "FAIL")^"\n");
-                   let newstate:ffiStateKeyExchange = {
-                    cske_guard = "CSKE";
-                    cske_config = config;
-                    cske_ks = ffiState.cscv_ks;
-                    cske_log = log;
-                    cske_lg = ffiState.cscv_lg;
-                    cske_ch = ffiState.cscv_ch;
-                    cske_n = n;
-                    cske_sc = sc;
-                    cske_sh = sh;
-                    cske_scb = scb;
-                   } in
-                   Correct(newstate))
-    | _ -> Error(AD_illegal_parameter,  "Unsupported sh_protocol_version")
-  
-  
-val ffiHandleCertificateVerify12:  ffiState:ffiStateCertificateVerify -> header:cbytes -> record:cbytes -> ffiStateKeyExchange
-let ffiHandleCertificateVerify12 ffiState header record =
-  let h = abytes header in
-  let r = abytes record in
-  match ffiHandleCertificateVerifyWorker12 ffiState h r with
-  | Error (x,z) -> IO.print_string (z^"\n"); failwith "error"
-  | Correct (x) -> x
-    
-    
-(*****************************************************************************************)
-type ffiStateServerHelloDone = {
-    cssd_guard: string;
-    cssd_config: config;
-    cssd_ks: ks;
-    cssd_log: bytes;
-    cssd_lg: HandshakeLog.log;
-    cssd_ch: HandshakeMessages.ch;
-    cssd_n:nego;
-    cssd_sc:HandshakeMessages.crt;
-    cssd_scb: bytes;
-    cssd_sh:HandshakeMessages.sh;
-    cssd_ske:HandshakeMessages.ske;
-    cssd_skeb:bytes;
-    }
-    
-val ffiHandleServerKeyExchangeWorker: ffiState:ffiStateKeyExchange -> header:bytes -> record:bytes -> (result (ffiStateServerHelloDone))
-let ffiHandleServerKeyExchangeWorker ffiState header record =
-  let _ = (if not (ffiState.cske_guard = "CSKE") then IO.print_string ("Incorrect cske_guard "^ffiState.cske_guard^"\n")) in
-  let _ = (if not (ffiState.cske_n.n_protocol_version = TLS_1p2) then IO.print_string ("This call is for TLS 1.2 only\n")) in
-  let config = ffiState.cske_config in
-  let log = ffiState.cske_log in
-  let sh = ffiState.cske_sh in
-  let n = ffiState.cske_n in
-  let pv = n.n_protocol_version in
-  let cs = n.n_cipher_suite in
-  let CipherSuite kex sa ae = cs in
-  let (ServerKeyExchange(ske),skeb) = recvHSRecord2 header record pv kex log in
-  let newstate:ffiStateServerHelloDone = {
-        cssd_guard = "CSSD";
-        cssd_config = config;
-        cssd_ks = ffiState.cske_ks;
-        cssd_log = log;
-        cssd_lg = ffiState.cske_lg;
-        cssd_ch = ffiState.cske_ch;
-        cssd_n = n;
-        cssd_sc = ffiState.cske_sc;
-        cssd_sh = ffiState.cske_sh;
-        cssd_scb = ffiState.cske_scb;
-        cssd_sh = sh;
-        cssd_ske = ske;
-        cssd_skeb = skeb;
-        } in
-    Correct(newstate)
-  
-val ffiHandleServerKeyExchange:  ffiState:ffiStateKeyExchange -> header:cbytes -> record:cbytes -> ffiStateServerHelloDone
-let ffiHandleServerKeyExchange ffiState header record =
-  let h = abytes header in
-  let r = abytes record in
-  match ffiHandleServerKeyExchangeWorker ffiState h r with
-  | Error (x,z) -> IO.print_string (z^"\n"); failwith "error"
-  | Correct (x) -> x
-    
-(*****************************************************************************************)
-type ffiStateClientKeyExchange = {
-    csck_guard: string;
-    csck_config: config;
-    csck_log: bytes;
-    csck_lg: HandshakeLog.log;
-    csck_n:nego;
-    csck_ks: ks;
-    csck_cke: HandshakeMessages.cke;
-    csck_ckeb: bytes;
-}
-
-val ffiHandleServerHelloDoneWorker: ffiState:ffiStateServerHelloDone -> header:bytes -> record:bytes -> (result (ffiStateClientKeyExchange))
-let ffiHandleServerHelloDoneWorker ffiState header record =
-  let _ = (if not (ffiState.cssd_guard = "CSSD") then IO.print_string ("Incorrect cssd_guard "^ffiState.cssd_guard^"\n")) in
-  let _ = (if not (ffiState.cssd_n.n_protocol_version = TLS_1p2) then IO.print_string ("This call is for TLS 1.2 only\n")) in
-  let config = ffiState.cssd_config in
-  let log = ffiState.cssd_log in
-  let lg = ffiState.cssd_lg in
-  let n = ffiState.cssd_n in
-  let pv = n.n_protocol_version in
-  let cs = n.n_cipher_suite in
-  let CipherSuite kex sa ae = cs in
-  let (ServerHelloDone,shdb) = recvHSRecord2 header record pv kex log in
-
-  let ske = ffiState.cssd_ske in
-  let skeb = ffiState.cssd_skeb in
-  let tbs = kex_s_to_bytes ske.ske_kex_s in
-  let sigv = ske.ske_sig in
-  let ch = ffiState.cssd_ch in
-  let cr = ch.ch_client_random in
-  let sh = ffiState.cssd_sh in
-  let sr = sh.sh_server_random in
-  let scb = ffiState.cssd_scb in
-  let ks = ffiState.cssd_ks in
-  let sc = ffiState.cssd_sc in
-  let (ClientKeyExchange cke,ckeb) = 
-     match
-       Handshake.processServerHelloDone config n ks lg
-      	[(Certificate sc,scb);(ServerKeyExchange ske, skeb);(ServerHelloDone,shdb)]
-	[] with
-     | Correct [x] -> x 
-     | Error (y,z) -> failwith (z ^ "\n") in
-   let newstate:ffiStateClientKeyExchange = {
-    csck_guard = "CSCK";
-    csck_config = config;
-    csck_log = log;
-    csck_lg = lg;
-    csck_n = n;
-    csck_ks = ffiState.cssd_ks;
-    csck_cke = cke;
-    csck_ckeb = ckeb;
-   } in
-   Correct(newstate)
-
-val ffiHandleServerHelloDone:  ffiState:ffiStateServerHelloDone -> header:cbytes -> record:cbytes -> ffiStateClientKeyExchange
-let ffiHandleServerHelloDone ffiState header record =
-  let h = abytes header in
-  let r = abytes record in
-  match ffiHandleServerHelloDoneWorker ffiState h r with
-  | Error (x,z) -> IO.print_string (z^"\n"); failwith "error"
-  | Correct (x) -> (x)
-    
-(*****************************************************************************************)
-let sendRecord2 pv ct msg str = 
-  let r = Record.makePacket ct pv msg in
-  (*let _ = (match ct with
-  | Content.Application_data ->   IO.print_string ("Sending Data("^str^")\n")
-  | Content.Handshake ->   IO.print_string ("Sending HS("^str^")\n")
-  | Content.Change_cipher_spec ->   IO.print_string ("Sending CCS\n")
-  | Content.Alert ->   IO.print_string ("Sending Alert("^str^")\n")) in  *)
-  r
- 
-let sendHSRecord2 pv (m,b) = 
-  let str = string_of_handshakeMessage m in
-  sendRecord2 pv Content.Handshake b str
-
-val ffiPrepareClientKeyExchange:  ffiState:ffiStateClientKeyExchange -> (cbytes * ffiStateClientKeyExchange)
-let ffiPrepareClientKeyExchange ffiState =
-  let _ = (if not (ffiState.csck_guard = "CSCK") then IO.print_string ("Incorrect csck_guard "^ffiState.csck_guard^"\n")) in
-  let _ = (if not (ffiState.csck_n.n_protocol_version = TLS_1p2) then IO.print_string ("This call is for TLS 1.2 only\n")) in
-  let n = ffiState.csck_n in
-  let pv = n.n_protocol_version in
-  let cke = ffiState.csck_cke in
-  let ckeb = ffiState.csck_ckeb in
-  let r = Record.makePacket Content.Handshake pv ckeb in
-  (get_cbytes r, ffiState)
-
-(*****************************************************************************************)
-type ffiStateHandshake = {
-    cshs_guard: string;
-    cshs_config: config;
-    cshs_log: bytes;
-    cshs_lg: HandshakeLog.log;
-    cshs_ks: ks;
-    cshs_n:nego;
-    cshs_wr: (StatefulLHAE.writer TestClient.id);
-    cshs_rd: (StatefulLHAE.reader TestClient.id);
-    cshs_efinb: bytes;
-    cshs_str: string;
-}
-
-
-val ffiPrepareChangeCipherSpec:  ffiState:ffiStateClientKeyExchange -> (cbytes * ffiStateHandshake)
-let ffiPrepareChangeCipherSpec ffiState =
-  let _ = (if not (ffiState.csck_guard = "CSCK") then IO.print_string ("Incorrect csck_guard "^ffiState.csck_guard^"\n")) in
-  let _ = (if not (ffiState.csck_n.n_protocol_version = TLS_1p2) then IO.print_string ("This call is for TLS 1.2 only\n")) in
-  let log = ffiState.csck_lg in
-  let n = ffiState.csck_n in
-  let pv = n.n_protocol_version in
-  let ks = ffiState.csck_ks in
-  let ems = n.n_extensions.ne_extended_ms in
-  let sal = n.n_extensions.ne_signature_algorithms in
-  
-  let lb = HandshakeLog.getBytes log in
-  (* if ems then IO.print_string " ***** USING EXTENDED MASTER SECRET ***** \n";
-//  IO.print_string ("master secret:"^(Platform.Bytes.print_bytes ms)^"\n"); *)
-  let (ck, civ, sk, siv) = KeySchedule.ks_12_get_keys ks in
-  (*IO.print_string ("client AES_GCM write key:"^(Platform.Bytes.print_bytes ck)^"\n");
-  IO.print_string ("client AES_GCM salt: iv:"^(Platform.Bytes.print_bytes civ)^"\n");
-  IO.print_string ("server AES_GCM write key:"^(Platform.Bytes.print_bytes sk)^"\n");
-  IO.print_string ("server AES_GCM salt:"^(Platform.Bytes.print_bytes siv)^"\n"); *)
-  let wr = TestClient.encryptor_TLS12_AES_GCM_128_SHA256 ck civ in
-  let rd = TestClient.decryptor_TLS12_AES_GCM_128_SHA256 sk siv in
-
-  let (Finished cfin, cfinb) = Handshake.prepareClientFinished ks log in
-  let str = string_of_handshakeMessage (Finished cfin) in 
-  let efinb = TestClient.encryptRecord_TLS12_AES_GCM_128_SHA256 wr Content.Handshake cfinb in
-  let r = sendRecord2 pv Content.Change_cipher_spec HandshakeMessages.ccsBytes "Client" in
-  let newstate:ffiStateHandshake = {
-    cshs_guard="CSHS";
-    cshs_config=ffiState.csck_config;
-    cshs_log=ffiState.csck_log;
-    cshs_lg=log;
-    cshs_ks=ffiState.csck_ks;
-    cshs_n=ffiState.csck_n;
-    cshs_wr = wr;
-    cshs_rd = rd;
-    cshs_efinb = efinb;
-    cshs_str = str;
-  } in
-  (get_cbytes r, newstate)
-  
-val ffiPrepareHandshake:  ffiState:ffiStateHandshake -> (cbytes * ffiStateHandshake)
-let ffiPrepareHandshake ffiState =
-  let _ = (if not (ffiState.cshs_guard = "CSHS") then IO.print_string ("Incorrect cshs_guard "^ffiState.cshs_guard^"\n")) in
-  let _ = (if not (ffiState.cshs_n.n_protocol_version = TLS_1p2) then IO.print_string ("This call is for TLS 1.2 only\n")) in
-  let n = ffiState.cshs_n in
-  let pv = n.n_protocol_version in
-  let r = sendRecord2 pv Content.Handshake ffiState.cshs_efinb ffiState.cshs_str in
-  (get_cbytes r, ffiState)
-
-(*****************************************************************************************)
-val ffiHandleChangeCipherSpecWorker: ffiState:ffiStateHandshake -> header:bytes -> record:bytes -> (result (ffiStateHandshake))
-let ffiHandleChangeCipherSpecWorker ffiState header record =
-  let _ = (if not (ffiState.cshs_guard = "CSHS") then IO.print_string ("Incorrect cske_guard "^ffiState.cshs_guard^"\n")) in
-  let _ = (if not (ffiState.cshs_n.n_protocol_version = TLS_1p2) then IO.print_string ("This call is for TLS 1.2 only\n")) in
-  let config = ffiState.cshs_config in
-  let log = ffiState.cshs_log in
-  let n = ffiState.cshs_n in
-  let pv = n.n_protocol_version in
-  let cs = n.n_cipher_suite in
-  let CipherSuite kex sa ae = cs in
-  let c = check_read header record pv in
-  match c with
-  | Error (x,z) -> IO.print_string (z^"\n"); Error (x,z)
-  | Correct(Content.Change_cipher_spec,rpv,pl) -> Correct(ffiState)
-  
-val ffiHandleChangeCipherSpec:  ffiState:ffiStateHandshake -> header:cbytes -> record:cbytes -> ffiStateHandshake
-let ffiHandleChangeCipherSpec ffiState header record =
-  let h = abytes header in
-  let r = abytes record in
-  match ffiHandleChangeCipherSpecWorker ffiState h r with
-  | Error (x,z) -> IO.print_string (z^"\n"); failwith "error"
-  | Correct (x) -> x
-    
-(*****************************************************************************************)
-let recvEncHSRecord2 header record pv kex log rd = 
-  let Correct(Content.Handshake,_,cipher) = check_read header record pv in
-  let payload = TestClient.decryptRecord_TLS12_AES_GCM_128_SHA256 rd Content.Handshake cipher in
-  let Correct (rem,hsm) = Handshake.parseHandshakeMessages (Some pv) (Some kex) payload in
-  let [(hs_msg,to_log)] = hsm in
-  IO.print_string ("Received HS("^(string_of_handshakeMessage hs_msg)^")\n");
-  let logged = handshakeMessageBytes (Some pv) hs_msg in
-  IO.print_string ("Logged message = Parsed message? ");
-  if (Platform.Bytes.equalBytes logged to_log) then IO.print_string "yes\n" else IO.print_string "no\n";
-  hs_msg,to_log
-
-val ffiHandleServerFinishedWorker: ffiState:ffiStateHandshake -> header:bytes -> record:bytes -> (result (ffiStateHandshake))
-let ffiHandleServerFinishedWorker ffiState header record =
-  let _ = (if not (ffiState.cshs_guard = "CSHS") then IO.print_string ("Incorrect cske_guard "^ffiState.cshs_guard^"\n")) in
-  let _ = (if not (ffiState.cshs_n.n_protocol_version = TLS_1p2) then IO.print_string ("This call is for TLS 1.2 only\n")) in
-  let config = ffiState.cshs_config in
-  let log = ffiState.cshs_log in
-  let n = ffiState.cshs_n in
-  let pv = n.n_protocol_version in
-  let cs = n.n_cipher_suite in
-  let CipherSuite kex sa ae = cs in
-  let rd = ffiState.cshs_rd in
-  let ks = ffiState.cshs_ks in
-  let lg = ffiState.cshs_lg in
-  let (Finished(sfin),sfinb) = recvEncHSRecord2 header record pv kex lg rd in
-  let Correct svd = Handshake.processServerFinished ks lg (Finished sfin, sfinb) in
-  (*IO.print_string ("Recd fin = expected fin? ");
-  if (Platform.Bytes.equalBytes sfin.fin_vd svd) then IO.print_string "yes\n" else IO.print_string "no\n"; *)
-  Correct(ffiState)
-  
-val ffiHandleServerFinished:  ffiState:ffiStateHandshake -> header:cbytes -> record:cbytes -> ffiStateHandshake
-let ffiHandleServerFinished ffiState header record =
-  let h = abytes header in
-  let r = abytes record in
-  match ffiHandleServerFinishedWorker ffiState h r with
-  | Error (x,z) -> IO.print_string (z^"\n"); failwith "error"
-  | Correct (x) -> x
-    
-(*****************************************************************************************)
-val ffiPrepareSend:  ffiState:ffiStateHandshake -> cbytes -> cbytes
-let ffiPrepareSend ffiState payload =
-  let _ = (if not (ffiState.cshs_guard = "CSHS") then IO.print_string ("Incorrect cshs_guard "^ffiState.cshs_guard^"\n")) in
-  let _ = (if not (ffiState.cshs_n.n_protocol_version = TLS_1p2) then IO.print_string ("This call is for TLS 1.2 only\n")) in
-  let n = ffiState.cshs_n in
-  let pv = n.n_protocol_version in
-  let wr = ffiState.cshs_wr in
-  let msg = TestClient.encryptRecord_TLS12_AES_GCM_128_SHA256 wr Content.Application_data (utf8 payload) in
-  let r = sendRecord2 pv Content.Application_data msg "Send" in
-  get_cbytes r
-(*****************************************************************************************)
-   
-val ffiHandleReceiveWorker: ffiState:ffiStateHandshake -> header:bytes -> record:bytes -> (result (bytes))
-let ffiHandleReceiveWorker ffiState header record =
-  let _ = (if not (ffiState.cshs_guard = "CSHS") then IO.print_string ("Incorrect cske_guard "^ffiState.cshs_guard^"\n")) in
-  let _ = (if not (ffiState.cshs_n.n_protocol_version = TLS_1p2) then IO.print_string ("This call is for TLS 1.2 only\n")) in
-  let config = ffiState.cshs_config in
-  let n = ffiState.cshs_n in
-  let pv = n.n_protocol_version in
-  let rd = ffiState.cshs_rd in
-  let c = check_read header record pv in
-  match c with
-  | Error (x,z) -> IO.print_string (z^"\n"); Error (x,z)
-  | Correct(Content.Application_data,_,cipher) -> 
-      let cleartext = TestClient.decryptRecord_TLS12_AES_GCM_128_SHA256 rd Content.Application_data cipher in
-      Correct (cleartext)
-      
-  
-val ffiHandleReceive:  ffiState:ffiStateHandshake -> header:cbytes -> record:cbytes -> cbytes
-let ffiHandleReceive ffiState header record =
-  let h = abytes header in
-  let r = abytes record in
-  match ffiHandleReceiveWorker ffiState h r with
-  | Error (x,z) -> IO.print_string (z^"\n"); failwith "error"
-  | Correct (x) -> get_cbytes x 
-
 (*****************************************************************************************)
 
 type cookie = FFICallbacks.cookie
@@ -656,9 +177,9 @@ let rec really_read_rec prev cookie len =
 
 private let really_read = really_read_rec empty_bytes
 
-val read: cookie -> protocolVersion -> 
+val recvRecordCallback: cookie -> protocolVersion -> 
   (result (Content.contentType * protocolVersion * b:bytes { length b <= max_TLSCiphertext_fragment_length}))
-let read cookie pv =
+let recvRecordCallback cookie pv =
   match really_read cookie 5 with 
   | Correct header -> (
       match Record.parseHeader header with  
@@ -669,9 +190,25 @@ let read cookie pv =
       | Error e             -> Error e )
   | Error e                 -> Error e
 
+let hsbuf = alloc ([] <: list (hs_msg * bytes))
+
+let recvHSRecordCallback12 cookie pv kex log = 
+  let (hs_msg, to_log) = match !hsbuf with
+    | [] -> 
+      let Correct(ct,rpv,pl) = recvRecordCallback cookie pv in
+      let hsml = match Handshake.parseHandshakeMessages (Some pv) (Some kex) pl with
+      	         | Correct(_,hsml) -> hsml | Error (y,z) -> IO.print_string(z); failwith "parseHSM failed" in
+      let (hs_msg, to_log)::r = hsml in
+      hsbuf := r; (hs_msg, to_log)
+    | h::t -> hsbuf := t; h in
+  IO.print_string ("Received HS("^(string_of_handshakeMessage hs_msg)^")\n");
+  let logged = handshakeMessageBytes (Some pv) hs_msg in
+  IO.print_string ("Logged message = Parsed message? ");
+  if (Platform.Bytes.equalBytes logged to_log) then IO.print_string "yes\n" else IO.print_string "no\n";
+  (hs_msg,to_log)
   
 let recvHSRecordCallback cookie pv kex log = 
-  let Correct(Content.Handshake,rpv,pl) = read cookie pv in
+  let Correct(Content.Handshake,rpv,pl) = recvRecordCallback cookie pv in
   match Handshake.parseHandshakeMessages (Some pv) (Some kex) pl with
   | Correct (rem,[(hs_msg,to_log)]) -> 
      	    (IO.print_string ("Received HS("^(string_of_handshakeMessage hs_msg)^")\n");
@@ -679,22 +216,194 @@ let recvHSRecordCallback cookie pv kex log =
   | Error (x,z) -> IO.print_string (z^"\n"); failwith "error"
   
  let recvEncHSRecordCallback cookie pv kex log rd = 
-  let Correct(Content.Application_data,_,cipher) = read cookie pv in
+  let Correct(Content.Application_data,_,cipher) = recvRecordCallback cookie pv in
   let payload = decryptRecord_TLS13_AES_GCM_128_SHA256 rd Content.Handshake cipher in
   let Correct (rem,hsm) = Handshake.parseHandshakeMessages (Some pv) (Some kex) payload in 
   let [(hs_msg,to_log)] = hsm in
   IO.print_string ("Received HS("^(string_of_handshakeMessage hs_msg)^")\n");
   hs_msg, log @| to_log	      
+  
+let recvEncHSRecordCallback12 cookie pv kex log rd = 
+  let Correct(Content.Handshake,_,cipher) = recvRecordCallback cookie pv in
+  let payload = TestClient.decryptRecord_TLS12_AES_GCM_128_SHA256 rd Content.Handshake cipher in
+  let Correct (rem,hsm) = Handshake.parseHandshakeMessages (Some pv) (Some kex) payload in
+  let [(hs_msg,to_log)] = hsm in
+  IO.print_string ("Received HS("^(string_of_handshakeMessage hs_msg)^")\n");
+  let logged = handshakeMessageBytes (Some pv) hs_msg in
+  IO.print_string ("Logged message = Parsed message? ");
+  if (Platform.Bytes.equalBytes logged to_log) then IO.print_string "yes\n" else IO.print_string "no\n";
+  hs_msg,to_log  
 
 let sendRecordCallback cookie pv ct msg str = 
   let r = Record.makePacket ct pv msg in
   let Correct _ = sendTcpPacket cookie r in
   IO.print_string ("Sending "^Content.ctToString ct^"Data("^str^")\n")
 
+let sendHSRecordCallback12 cookie pv (m,b) = 
+  let str = string_of_handshakeMessage m in
+  sendRecordCallback cookie pv Content.Handshake b str
+
 let sendHSRecordCallback cookie pv hs_msg log = 
   let (str,hs,log) = makeHSRecord pv hs_msg log in
   sendRecordCallback cookie pv Content.Handshake hs str;
   log
+    
+let makePacket pv ct msg str = 
+  let r = Record.makePacket ct pv msg in
+  (*let _ = (match ct with
+  | Content.Application_data ->   IO.print_string ("Sending Data("^str^")\n")
+  | Content.Handshake ->   IO.print_string ("Sending HS("^str^")\n")
+  | Content.Change_cipher_spec ->   IO.print_string ("Sending CCS\n")
+  | Content.Alert ->   IO.print_string ("Sending Alert("^str^")\n")) in  *)
+  r
+  
+let rec really_check buf len = 
+    let lb = length buf in
+    if len = 0 then Correct buf
+    else if len = lb then Correct buf
+    else Error(AD_illegal_parameter,  "Unexpected buffer length")
+  
+let check_read header record pv =
+  match really_check header 5 with 
+  | Correct header -> (
+      match Record.parseHeader header with  (* contenType protocolVersion length *)
+      | Correct (ct,pv,len) -> (
+         match really_check record len with
+         | Correct payload  -> Correct (ct,pv,payload)
+         | Error e          -> Error e )
+      | Error e             -> Error e )
+  | Error e                 -> Error e
+  
+(*****************************************************************************************)
+
+type ffiStateClient12 = {
+    cscc_guard: string;
+    cscc_config: config;
+    cscc_pv: protocolVersion;
+    cscc_wr: (StatefulLHAE.writer TestClient.id);
+    cscc_rd: (StatefulLHAE.reader TestClient.id);
+}
+
+let recvCCSRecordCallback cookie pv = 
+  let Correct(Content.Change_cipher_spec,_,ccs) = recvRecordCallback cookie pv in
+  IO.print_string "Received CCS\n";
+  ccs
+
+val ffiConnect12: ffiState:ffiStateClientHello -> cookie:cookie -> ffiStateClient12
+let ffiConnect12 ffiState cookie =
+  let _ = (if not (ffiState.csch_guard = "CSCH") then IO.print_string ("Incorrect csch_guard "^ffiState.csch_guard^"\n")) in
+  let config = ffiState.csch_config in
+  let rid = new_region root in
+  let log = HandshakeLog.create #rid in
+
+  let ks, cr = KeySchedule.create #rid Client in
+  let (ClientHello ch,chb) = Handshake.prepareClientHello config ks log None None in
+  let pv = ch.ch_protocol_version in 
+  let kex = TLSConstants.Kex_ECDHE in
+
+  sendHSRecordCallback12 cookie pv (ClientHello ch,chb);
+
+  let (ServerHello(sh),shb) = recvHSRecordCallback12 cookie pv kex log in
+  
+  let Correct (n,None) = Handshake.processServerHello config ks log None ch (ServerHello(sh),shb) in
+
+  let pv = n.n_protocol_version in
+  let cs = n.n_cipher_suite in
+  let CipherSuite kex sa ae = cs in
+  let ems = n.n_extensions.ne_extended_ms in
+  let sal = n.n_extensions.ne_signature_algorithms in
+
+  let (Certificate(sc),scb) = recvHSRecordCallback12 cookie pv kex log in
+  IO.print_string ("Certificate validation status = " ^
+    (if Cert.validate_chain sc.crt_chain true config.peer_name config.ca_file then
+      "OK" else "FAIL")^"\n");
+
+  let (ServerKeyExchange(ske),skeb) = recvHSRecordCallback12 cookie pv kex log in
+  let (ServerHelloDone,shdb) = recvHSRecordCallback12 cookie pv kex log in
+
+  let tbs = kex_s_to_bytes ske.ske_kex_s in
+  let sigv = ske.ske_sig in
+  let cr = ch.ch_client_random in
+  let sr = sh.sh_server_random in
+  let (ClientKeyExchange cke,ckeb) = 
+     match
+       Handshake.processServerHelloDone config n ks log
+      	[(Certificate sc,scb);(ServerKeyExchange ske, skeb);(ServerHelloDone,shdb)]
+	[] with
+     | Correct [x] -> x 
+     | Error (y,z) -> failwith (z ^ "\n") in
+
+  sendHSRecordCallback12 cookie pv (ClientKeyExchange cke,ckeb);
+
+  let lb = HandshakeLog.getBytes log in
+  if ems then IO.print_string " ***** USING EXTENDED MASTER SECRET ***** \n";
+//  IO.print_string ("master secret:"^(Platform.Bytes.print_bytes ms)^"\n");
+  let (ck, civ, sk, siv) = KeySchedule.ks_12_get_keys ks in
+  IO.print_string ("client AES_GCM write key:"^(Platform.Bytes.print_bytes ck)^"\n");
+  IO.print_string ("client AES_GCM salt: iv:"^(Platform.Bytes.print_bytes civ)^"\n");
+  IO.print_string ("server AES_GCM write key:"^(Platform.Bytes.print_bytes sk)^"\n");
+  IO.print_string ("server AES_GCM salt:"^(Platform.Bytes.print_bytes siv)^"\n");
+  let wr = TestClient.encryptor_TLS12_AES_GCM_128_SHA256 ck civ in
+  let rd = TestClient.decryptor_TLS12_AES_GCM_128_SHA256 sk siv in
+
+  let (Finished cfin, cfinb) = Handshake.prepareClientFinished ks log in
+  let str = string_of_handshakeMessage (Finished cfin) in 
+  let efinb = TestClient.encryptRecord_TLS12_AES_GCM_128_SHA256 wr Content.Handshake cfinb in
+
+  sendRecordCallback cookie pv Content.Change_cipher_spec HandshakeMessages.ccsBytes "Client";
+  sendRecordCallback cookie pv Content.Handshake efinb str;
+
+  let _ = recvCCSRecordCallback cookie pv in
+  let (Finished(sfin),sfinb) = recvEncHSRecordCallback12 cookie pv kex log rd in
+  let Correct svd = Handshake.processServerFinished ks log (Finished sfin, sfinb) in
+
+
+  IO.print_string ("Recd fin = expected fin? ");
+  if (Platform.Bytes.equalBytes sfin.fin_vd svd) then IO.print_string "yes\n" else IO.print_string "no\n";
+  let newstate:ffiStateClient12 = {
+    cscc_guard="CSCC";
+    cscc_config=config;
+    cscc_pv=pv;
+    cscc_wr = wr;
+    cscc_rd = rd;
+  } in
+  newstate
+
+  
+val ffiPrepareSend12:  ffiState:ffiStateClient12 -> cbytes -> cbytes
+let ffiPrepareSend12 ffiState payload =
+  let _ = (if not (ffiState.cscc_guard = "CSHS") then IO.print_string ("Incorrect cscc_guard "^ffiState.cscc_guard^"\n")) in
+  let _ = (if not (ffiState.cscc_pv = TLS_1p2) then IO.print_string ("This call is for TLS 1.2 only\n")) in
+  let pv = ffiState.cscc_pv in
+  let wr = ffiState.cscc_wr in
+  let msg = TestClient.encryptRecord_TLS12_AES_GCM_128_SHA256 wr Content.Application_data (utf8 payload) in
+  let r = makePacket pv Content.Application_data msg "Send" in
+  get_cbytes r
+   
+val ffiHandleReceiveWorker12: ffiState:ffiStateClient12 -> header:bytes -> record:bytes -> (result (bytes))
+let ffiHandleReceiveWorker12 ffiState header record =
+  let _ = (if not (ffiState.cscc_guard = "CSCC") then IO.print_string ("Incorrect cscc_guard "^ffiState.cscc_guard^"\n")) in
+  let _ = (if not (ffiState.cscc_pv = TLS_1p2) then IO.print_string ("This call is for TLS 1.2 only\n")) in
+  let config = ffiState.cscc_config in
+  let pv = ffiState.cscc_pv in
+  let rd = ffiState.cscc_rd in
+  let c = check_read header record pv in
+  match c with
+  | Error (x,z) -> IO.print_string (z^"\n"); Error (x,z)
+  | Correct(Content.Application_data,_,cipher) -> 
+      let cleartext = TestClient.decryptRecord_TLS12_AES_GCM_128_SHA256 rd Content.Application_data cipher in
+      Correct (cleartext)
+      
+  
+val ffiHandleReceive12:  ffiState:ffiStateClient12 -> header:cbytes -> record:cbytes -> cbytes
+let ffiHandleReceive12 ffiState header record =
+  let h = abytes header in
+  let r = abytes record in
+  match ffiHandleReceiveWorker12 ffiState h r with
+  | Error (x,z) -> IO.print_string (z^"\n"); failwith "error"
+  | Correct (x) -> get_cbytes x 
+  
+(*****************************************************************************************)
 
 type ffiStateClient13 = {
     cscl_guard: string;
@@ -777,7 +486,7 @@ let ffiPrepareSend13 ffiState payload =
   let pv = ffiState.cscl_pv in
   let dwr = ffiState.cscl_dwr in
   let msg = encryptRecord_TLS13_AES_GCM_128_SHA256 dwr Content.Application_data (utf8 payload) in
-  let r = sendRecord2 pv Content.Application_data msg "Send" in
+  let r = makePacket pv Content.Application_data msg "Send" in
   get_cbytes r
 
   
